\subsection{Solving Systems Using LU}

Given:

\[
    A = LU,
    \quad
    Ax = b,
\]

we solve:

\[
    LUx = b.
\]

Let:

\[
    Ux = y.
\]

First solve:

\[
    Ly = b.
\]

Since $L$ is lower triangular, use forward substitution.

%------------------------------------------------

\subsubsection*{Example}

Let:

\[
    L =
    \begin{bmatrix}
        1 & 0 \\
        2 & 1
    \end{bmatrix},
    \quad
    U =
    \begin{bmatrix}
        2 & 3 \\
        0 & 1
    \end{bmatrix},
    \quad
    b =
    \begin{bmatrix}
        5 \\
        11
    \end{bmatrix}.
\]

Step 1: Solve $Ly = b$.

\[
    \begin{bmatrix}
        1 & 0 \\
        2 & 1
    \end{bmatrix}
    \begin{bmatrix}
        y_1 \\
        y_2
    \end{bmatrix}
    =
    \begin{bmatrix}
        5 \\
        11
    \end{bmatrix}.
\]

From first row:

\[
    y_1 = 5.
\]

Second row:

\[
    2(5) + y_2 = 11
    \Rightarrow y_2 = 1.
\]

Thus:

\[
    y =
    \begin{bmatrix}
        5 \\
        1
    \end{bmatrix}.
\]

Step 2: Solve $Ux = y$.

\[
    \begin{bmatrix}
        2 & 3 \\
        0 & 1
    \end{bmatrix}
    \begin{bmatrix}
        x_1 \\
        x_2
    \end{bmatrix}
    =
    \begin{bmatrix}
        5 \\
        1
    \end{bmatrix}.
\]

From second row:

\[
    x_2 = 1.
\]

First row:

\[
    2x_1 + 3(1) = 5
    \Rightarrow x_1 = 1.
\]

\begin{conceptbox}
    LU reduces solving $Ax=b$ to two simpler triangular systems.
\end{conceptbox}