\subsection{The Normal Equations}

From orthogonality:

\[
    A^T (b - Ax) = 0.
\]

Rearrange:

\[
    A^T A x = A^T b.
\]

\begin{conceptbox}
    The equation
    \[
        A^T A x = A^T b
    \]
    is called the normal equation.
\end{conceptbox}

%------------------------------------------------
\subsubsection*{Properties}

\begin{itemize}
    \item $A^T A$ is symmetric.
    \item If columns of $A$ are independent,
          $A^T A$ is invertible.
\end{itemize}

Thus:

\[
    x = (A^T A)^{-1} A^T b.
\]

%------------------------------------------------
\subsubsection*{Example (Line Fitting)}

Using earlier data:

\[
    A =
    \begin{bmatrix}
        1 & 1 \\
        2 & 1 \\
        3 & 1
    \end{bmatrix},
    \quad
    b =
    \begin{bmatrix}
        1 \\
        2 \\
        2
    \end{bmatrix}.
\]

Compute:

\[
    A^T A =
    \begin{bmatrix}
        14 & 6 \\
        6  & 3
    \end{bmatrix}.
\]

\[
    A^T b =
    \begin{bmatrix}
        11 \\
        5
    \end{bmatrix}.
\]

Solve:

\[
    \begin{bmatrix}
        14 & 6 \\
        6  & 3
    \end{bmatrix}
    \begin{bmatrix}
        m \\
        c
    \end{bmatrix}
    =
    \begin{bmatrix}
        11 \\
        5
    \end{bmatrix}.
\]

Solution:

\[
    m = \frac{1}{2}, \quad c = \frac{2}{3}.
\]